Add the 'RunBuilder'
This structure bundles the three objects necessary to define the
runner's journey: the sprints, the eaten cells, and the journey
itself. Each of these objects depends on the other so defining
them independently would be difficult.

The culmination of this change is the 'make_run', function which
constructs the RunBuilder corresponding to the runner's journey
of 'n' steps.

This change also fixes an earlier mistake where the maximum length
of a sprint was limited to '2p' rather than '2p + 1'

AngelDevil/Runner.lean
@@ -88,7 +88,8 @@ decreasing_by
 
 -- If the list constructed by 'sprint_partial' is not empty, the first element of the list will be 'rs'
 lemma sprint_partial_getElem_zero_of_nonnil (p ns : Nat) (start : Int × Int) (eaten : List (Int × Int)) (rs : RunState) :
-  (hnnil : sprint_partial p ns start eaten rs ≠ []) → (sprint_partial p ns start eaten rs)[0]'(List.length_pos_iff.mpr hnnil) = rs := by
+  (hnnil : sprint_partial p ns start eaten rs ≠ []) →
+  (sprint_partial p ns start eaten rs)[0]'(List.length_pos_iff.mpr hnnil) = rs := by
   intro hnnil
   -- Use the trick of starting with 'sprint_partial = sprint_partial' followed by 'nth_rw'
   -- to expand only the right-hand side. This allows us to easily do
@@ -136,6 +137,7 @@ lemma sprint_partial_cons_of_nonnil (p ns : Nat) (start : Int × Int) (eaten : L
     rw [dif_pos hterm]
   · rfl
 
+-- Any element of a partial sprint is close to the start of the sprint
 lemma sprint_partial_mem_close (p ns : Nat) (start : Int × Int) (eaten : List (Int × Int)) (rs : RunState) :
   ∀ x ∈ sprint_partial p ns start eaten rs, close p start (loc x) := by
   intro x hxmem
@@ -166,7 +168,7 @@ decreasing_by
 -- Later we will show that the cells corresponding to the beginning and end of
 -- the sprints can be used to construct an angel which escapes the Nice Devil.
 def sprint (p : Nat) (rs₀ : RunState) (eaten : List (Int × Int)) : List RunState :=
-  sprint_partial p 1 (loc rs₀) eaten rs₀
+  sprint_partial p 0 (loc rs₀) eaten rs₀
 
 -- If 'p' is positive, the sprint will not be empty
 -- Up to this point we have not needed this assumption, but it appears
@@ -178,11 +180,17 @@ lemma sprint_nonnil_of_ppos (p : Nat) (rs₀ : RunState) (eaten : List (Int × I
   split_ifs with hterm
   · contrapose! hterm
     constructor
-    · apply Nat.le_of_lt_add_one
-      apply Nat.add_one_lt_add_one_iff.mpr
-      linarith
+    · linarith
     · exact close_self p (loc rs₀)
   exact List.cons_ne_nil _ _
+
+lemma sprint_getElem_zero_of_ppos (p : Nat) (rs₀ : RunState) (eaten : List (Int × Int)) :
+  (ppos : 0 < p) → (sprint p rs₀ eaten)[0]'(by
+    apply List.length_pos_of_ne_nil
+    exact sprint_nonnil_of_ppos p rs₀ eaten ppos
+  ) = rs₀ :=
+  fun ppos ↦ sprint_partial_getElem_zero_of_nonnil p 0 (loc rs₀) eaten rs₀
+    (sprint_nonnil_of_ppos p rs₀ eaten ppos)
 
 -- Prove that the first and last cells in a sprint are "close"
 lemma sprint_close_first_last (p : Nat) (hpos : 0 < p) (rs₀ : RunState) (eaten : List (Int × Int)) :
@@ -192,7 +200,7 @@ lemma sprint_close_first_last (p : Nat) (hpos : 0 < p) (rs₀ : RunState) (eaten
   have hnnil := sprint_nonnil_of_ppos p rs₀ eaten hpos
   unfold sprint at *
   rw [List.head_eq_getElem_zero hnnil, sprint_partial_getElem_zero_of_nonnil]
-  · exact sprint_partial_mem_close p 1 (loc rs₀) eaten _ _ (List.getLast_mem hnnil)
+  · exact sprint_partial_mem_close p 0 (loc rs₀) eaten _ _ (List.getLast_mem hnnil)
   · assumption
 
 -- TODO: This might be useful more generally
@@ -207,3 +215,149 @@ def NoSteps (p : Nat) : Journey p where
   plimit := fun i ilt ↦ False.elim (Nat.not_lt_zero i ilt)
 
 lemma nosteps_steps (p : Nat) : steps (NoSteps p) = 0 := rfl
+
+/- The three different structures needed to define the runner's journey
+   have interdependencies that make them difficult to construct separately.
+   This structure will allow us to build all three together. -/
+structure RunBuilder (p : Nat) where
+  D : Devil
+  A : Journey p
+  eaten : List (Int × Int)
+  sprints : List (List RunState)
+  -- These bundled properties are somewhat eclectic
+  -- They are only included to facilitate the definition of 'build run' (below)
+  ppos : 0 < p
+  nonnil : ∀ s ∈ sprints, s ≠ []
+  samelen : steps A = sprints.length
+  origin : (snn : sprints ≠ []) →
+    (sprints[0]'(List.length_pos_of_ne_nil snn))[0]'(
+      List.length_pos_of_ne_nil (nonnil _ (List.getElem_mem (List.length_pos_of_ne_nil snn)))
+    ) = run_start
+  dest : (snn : sprints ≠ []) →
+    loc ((sprints.getLast snn).getLast (nonnil _ (List.getLast_mem snn))) = last A
+
+-- Get the final runner state from a run builder
+-- If we haven't had any sprints yet, use the default location and direction
+def final_state {p : Nat} (S : RunBuilder p) : RunState :=
+  if hlz : S.sprints.length = 0 then run_start else
+    (S.sprints.getLast (List.ne_nil_of_length_pos (Nat.pos_of_ne_zero hlz))).getLast
+    (S.nonnil _ (List.getLast_mem (List.ne_nil_of_length_pos (Nat.pos_of_ne_zero hlz))))
+
+-- If the list of sprints is empty, the final state of the run is the 'run_start'
+lemma final_state_of_sprints_nil {p : Nat} (S : RunBuilder p) (hnil : S.sprints = []) :
+  final_state S = run_start := by
+  unfold final_state
+  rw [dif_pos (List.length_eq_zero_iff.mpr hnil)]
+
+-- The location given by 'final_state' matches the last cell in the builder journey
+lemma final_state_loc_eq_journey_last {p : Nat} (S : RunBuilder p) :
+  loc (final_state S) = last S.A := by
+  unfold final_state
+  split_ifs with hlz
+  · exact (journey_last_of_steps_zero S.A (Eq.trans S.samelen hlz)).symm
+  · push_neg at hlz
+    exact S.dest (List.ne_nil_of_length_pos (Nat.pos_of_ne_zero hlz))
+
+-- Get the next sprint to be added to the builder
+def next_sprint {p : Nat} (S : RunBuilder p) : List RunState :=
+  sprint p (final_state S) S.eaten
+
+-- The initial state of the next sprint is the
+-- same as the final state of the builder
+lemma next_sprint_first_eq_builder_last {p : Nat} (S : RunBuilder p) :
+  final_state S = (next_sprint S)[0]'(by
+    apply List.length_pos_of_ne_nil
+    exact sprint_nonnil_of_ppos p (final_state S) S.eaten S.ppos
+  ) := by
+  unfold next_sprint
+  rw [sprint_getElem_zero_of_ppos]
+  exact S.ppos
+
+-- The last cell of the next sprint is "close" to the
+-- last cell of the builder journey.
+lemma next_sprint_last_close_builder_last {p : Nat} (S : RunBuilder p) :
+  close p (loc ((next_sprint S).getLast (sprint_nonnil_of_ppos p (final_state S) S.eaten S.ppos))) (last S.A) := by
+  rw [← final_state_loc_eq_journey_last]
+  nth_rw 2 [next_sprint_first_eq_builder_last S]
+  rw [close_comm, List.getElem_zero]
+  exact sprint_close_first_last _ S.ppos _ _
+
+-- Define the base case for our builder construction:
+-- The journey has no steps, there are no sprints, and the
+-- Devil has only eaten one cell
+def empty_builder (D : Devil) (p : Nat) (ppos : 0 < p) : RunBuilder p where
+  D := D
+  A := NoSteps p
+  eaten := [response D (NoSteps p)]
+  sprints := []
+  nonnil := fun _ hs ↦ False.elim (List.not_mem_nil hs)
+  ppos := ppos
+  samelen := by rw [nosteps_steps, List.length_nil]
+  origin := fun snn ↦ False.elim (snn rfl)
+  dest := fun snn ↦ False.elim (snn rfl)
+
+-- Construct the journey that corresponds to appending the
+-- last location of the next sprint
+def builder_journey_extend {p : Nat} (S : RunBuilder p) : Journey p :=
+  AppendJourney S.A (loc ((next_sprint S).getLast (sprint_nonnil_of_ppos p _ _ S.ppos)))
+  ((close_comm p _ _).mp (next_sprint_last_close_builder_last S))
+
+-- Why doesn't this theorem aleady exist?
+-- TODO: If this is needed elsewhere, move it into 'Basic.lean' or 'Util.lean'
+lemma list_singleton_ne_nil {α : Type} (x : α) : [x] ≠ [] := by
+  apply List.ne_nil_of_length_pos
+  rw [List.length_singleton]
+  norm_num
+
+/- Add another sprint to a 'RunBuilder'
+   Original this was named 'make_run' and used recursion to
+   directly construct the RunBuilder (rather than taking 'S' as an argument).
+   Unfortunately this caused timeouts, so now 'make_run' handles the recursion
+   separately and wraps 'extend_run' -/
+def extend_run (D : Devil) (p : Nat) (ppos : 0 < p) (S : RunBuilder p) : RunBuilder p:=
+  RunBuilder.mk D
+    (builder_journey_extend S)
+    (S.eaten ++ [response D (builder_journey_extend S)])
+    (S.sprints ++ [next_sprint S])
+    ppos
+    (by
+      intro s smem
+      rcases List.mem_append.mp smem with lhs | rhs
+      · exact RunBuilder.nonnil _ s lhs
+      · exact (List.mem_singleton.mp rhs) ▸ (sprint_nonnil_of_ppos p _ _ ppos)
+    )
+    (by
+      unfold builder_journey_extend
+      rw [append_steps, List.length_append, List.length_singleton]
+      exact Nat.add_one_inj.mpr (RunBuilder.samelen _)
+    )
+    (by
+      intro h
+      let sprints := S.sprints
+      let s := next_sprint S
+      by_cases hsn : sprints = []
+      · have h₀ : 0 < (sprints ++ [s]).length := by
+          rw [List.length_append, List.length_singleton]
+          exact Nat.add_one_pos _
+        have h₁ : sprints ++ [s] = [s] := by
+          rw [hsn, List.nil_append]
+        have h₂ : (sprints ++ [s])[0]'(h₀) = s :=
+          getElem_congr_coll h₁
+        rw [getElem_congr_coll h₂]
+        rw [← next_sprint_first_eq_builder_last _]
+        exact final_state_of_sprints_nil _ hsn
+      · rename' hsn => hsnn; push_neg at hsnn
+        rw [getElem_congr_coll (List.getElem_append_left (List.length_pos_of_ne_nil hsnn))]
+        exact RunBuilder.origin _ hsnn
+    )
+    (by
+      intro h
+      unfold builder_journey_extend
+      rw [append_last]; congr
+      rw [List.getLast_append_right (list_singleton_ne_nil _)]
+      rw [List.getLast_singleton (list_singleton_ne_nil _)]
+    )
+
+def make_run (D : Devil) (p n : Nat) (ppos : 0 < p) : RunBuilder p :=
+  if n = 0 then empty_builder D p ppos else
+  extend_run D p ppos (make_run D p (n - 1) ppos)
